\documentclass{article}
\usepackage{enumerate}
\begin{document}
\begin{enumerate}[A]
\item
\[
\textrm{prox }_\gamma f(x,x_0)=\textrm{arg min}_z\frac{1}{2\gamma}(z-x)^2+z^T\nabla f(x_0)=\textrm{arg min}_z\frac{1}{2\gamma}z^2-\frac{1}{\gamma}z^Tx+z^T\nabla f(x_0)=x-\gamma\nabla f(x_0)
\]

\item
\begin{eqnarray}
\textrm{prox}_{\frac{1}{\gamma}}l(x)&=&\textrm{arg min}_z\frac{\gamma}{2}(z-x)^2+\frac{1}{2}z^TPz-q^Tz\nonumber\\
&=&\textrm{arg min}_z\frac{1}{2}z^T(P+I\gamma)z-q^Tz-\gamma x^Tz\nonumber\\
&=&\textrm{arg min}_z \frac{1}{2}(z-(P+I\gamma)^{-1}(q+\gamma x))^T(P+I\lambda)(z-(P+I\gamma)^{-1}(q+\gamma x))\nonumber\\
&=&(P+I\gamma)^{-1}(q+\gamma x)\nonumber
\end{eqnarray}
\[
\textrm{negative loglikelihood}=\frac{1}{2}(y-Ax)^T\Omega^{-1}(y-Ax)=\frac{1}{2}y^T\Omega^{-1}y-x^TA^T\Omega^{-1}y+\frac{1}{2}x^TA^T\Omega^{-1}Ax
\]
\[
P=\Omega^{-1}
\]
\[
q=\Omega^{-1}Ax
\]
\[
r=\frac{1}{2}x^TA^T\Omega^{-1}Ax
\]
\item
\[
\textrm{prox }_\gamma\phi(x)=\textrm{arg min}_z \frac{1}{2\gamma}(z-x)^2+\tau|z|=\textrm{arg min}_z \frac{1}{2}(z-x)^2+\tau\gamma|z|=S_{\tau\gamma}(x)
\]
\end{enumerate}
\begin{enumerate}[A]
\item
\begin{eqnarray}
&&\textrm{arg min}_x l(x,x_0)+\phi(x)\nonumber\\
&=&\textrm{arg min}_x \frac{1}{2\gamma}(x-x_0)^2+x\nabla l(x_0)+\phi(x)\nonumber\\
&=&\textrm{arg min}_x \frac{1}{2\gamma}(x-x_0+\gamma\nabla l(x_0))^2+\phi(x)\nonumber\\
&=&\textrm{prox}_\gamma\phi(x_0-\gamma\nabla l(x_0))\nonumber
\end{eqnarray}
\item
\[
\nabla_\beta\frac{1}{2n}(y-X\beta)=\frac{1}{n}(X^TX\beta+X^Ty):=\Delta
\]
\begin{eqnarray}
\beta_{t+1}&=&\textrm{arg min}_{\beta_t} \frac{1}{2n}(y-X\beta_t)^2+\lambda|\beta_t|\nonumber\\
&=&\textrm{prox}_{\gamma}\lambda|\beta_t-\gamma\Delta|_{\beta_t}|\nonumber\\
&=&S_{\lambda\gamma}(\beta_t-\gamma\Delta)
\end{eqnarray}
\end{enumerate}
\end{document}