\documentclass{article}
\begin{document}
Define
\[
S_{1\lambda}(y)=\textrm{arg min}_{\theta\geq0}\frac{1}{2}\theta^2-(y-\lambda)\theta
\]

\[
S_{2\lambda}(y)=\textrm{arg min}_{\theta\leq0}\frac{1}{2}\theta^2-(y+\lambda)\theta
\]

Then $S_\lambda(y)$ is one of $S_{1\lambda}(y)$ and $S_{2\lambda}(y)$  which gives the smaller target function.
Assuming $\lambda>0$. When $y>\lambda$,
\[
S_{1\lambda}(y)=y-\lambda
\]
\[
S_{2\lambda}(y)=0
\]
\[
\frac{1}{2}S_{1\lambda}(y)^2-(y-\lambda)S_{1\lambda}(y)-\frac{1}{2}S_{2\lambda}(y)^2+(y+\lambda)S_{2\lambda}(y)=-\frac{1}{2}(y-\lambda)^2<0
\]
So $S_{\lambda}(y)=y-\lambda$

If $-\lambda<y<\lambda$
\[
S_{1\lambda}(y)=0
\]
\[
S_{2\lambda}(y)=0
\]

So $S_{\lambda}(y)=0$

If $y<\lambda$
\[
S_{1\lambda}(y)=0
\]
\[
S_{2\lambda}(y)=y+\lambda
\]
\[
\frac{1}{2}S_{1\lambda}(y)^2-(y-\lambda)S_{1\lambda}(y)-\frac{1}{2}S_{2\lambda}(y)^2+(y+\lambda)S_{2\lambda}(y)=\frac{1}{2}(y+\lambda)^2>0
\]
So $S_{\lambda}(y)=y+\lambda$
\end{document}